---
title: "Hilbert Transform"
---

## Representation of the Potential Gradient in the Complex Plane

Let $u$ and $v$ denote the real and imaginary parts of a complex-valued function of the complex variable $z = x + i y$, with $f(x + iy) = u(x,y) + iv(x,y)$. The functions $u$ and $v$ are real-valued and differentiable at every point in an open subset $\Omega \subset \mathbb{C}$. These functions map from $\mathbb{R}^2$ to $\mathbb{R}$.

A function $f: \mathbb{C} \to \mathbb{C}$, $f(z) = u + iv$, defined in a domain $\Omega$, is called _holomorphic_ if the real-valued functions $u(x,y)$ and $v(x,y)$ are continuously differentiable in $\Omega$, and their partial derivatives satisfy the relations
$$
\begin{align}
u_x & = +v_y, \\
u_y & = -v_x,
\end{align}
$$
at every point in $\Omega$. These are the _Cauchy-Riemann differential equations_ (CRD).

Consider a function $f: \mathbb{C} \mapsto \mathbb{C}$. We want to demonstrate that this function is complex differentiable and holomorphic.

Definition of the derivative:

$$
f'(z) = \lim_{ h \to 0 } \frac{f(z + h) - f(z)}{h}
$$
What does this limit mean by thinking of the real and imaginary parts separately? Let's replace $z$ with $x+iy$:
$$
f'(x +iy) = \lim_{ h \to 0 } \frac{f(x + iy + h) - f(x + iy)}{h}
$$
Now $h$ is also a complex number. Replace $h$ by $a + ib$ and take the limit as $a$ and $b$ together approach $0$:

$$
f'(x +iy) = \lim_{ (a,b) \to (0,0) } \frac{f(x + iy + a + ib) - f(x + iy)}{a + ib}
$$
Now introduce a new function $F: \mathbb{R}^{2} \mapsto \mathbb{C}$ that $F(x,y) = f(x + iy)$. $F$ is a function of two real variables, $f$ is a function of a single complex variable.

$$
f'(x +iy) = \lim_{ (a,b) \to (0,0) } \frac{F(x + a, y + b) - F(x, y)}{a + ib}
$$
If that limit exists, then it is equal to the same limit when we just restrict to moving aong the real axis, i.e., when we approach $(0,0)$ just along the real axis.
We set $b=0$ and write
$$
f'(x +iy) = \lim_{ a \to 0, b=0 } \frac{F(x + a, y + b) - F(x, y)}{a + ib}
$$
This is a restricted situation, but if the limit exists for $(a,b) \to (0,0)$ then this limit must also exist and approach to the same quantity.
$$
f'(x +iy) = \lim_{ a \to 0 } \frac{F(x + a, y) - F(x, y)}{a} = \frac{\partial F}{\partial x}(x,y)
$$
Now we repeat the same story and instead of restricting to the real axis we restrict to the imaginary axis.
$$
f'(x +iy) = \lim_{ a =\to= 0, b \to 0 } \frac{F(x + a, y + b) - F(x, y)}{a + ib}
$$
$$
f'(x +iy) = \lim_{ b \to 0 } \frac{F(x, y + b) - F(x, y)}{ib} = \frac{1}{i}\frac{\partial F}{\partial y}(x,y)
$$
If these limits are the same, then
$$
\frac{\partial F}{\partial x}(x,y) = \frac{1}{i} \frac{\partial F}{\partial y}(x,y)
$$
Now introduce two new functions: $u: \mathbb{R}^{2} \to \mathbb{R}$ and $v: \mathbb{R}^{2} \to \mathbb{R}$, such that
$$
F(x,y) = u(x,y) + i v(x,y)
$$
Now expand out the partial derivative
$$
\frac{\partial u}{\partial x} + i \frac{\partial v}{\partial x} = \frac{1}{i} \frac{\partial F}{\partial y}(x,y) = \frac{1}{i}\left( \frac{\partial u}{\partial y} + i \frac{\partial v}{\partial y} \right) = \left( \frac{1}{i}\frac{\partial u}{\partial y} + \frac{\partial v}{\partial y} \right)
$$
and equate the real and imaginary parts
$$
\frac{\partial u}{\partial x} = \frac{\partial v}{\partial y} \qquad \frac{1}{i} \frac{\partial u}{\partial y} = i \frac{\partial v}{\partial x}
$$
which become the _Cauchy-Riemann equations_
$$
\frac{\partial u}{\partial x} = \frac{\partial v}{\partial y} \qquad \frac{\partial u}{\partial y} = - \frac{\partial v}{\partial x}
$$
A function is called _holomorphic_ when these equation are satisfied. The stronger condition however is that  $u$ and $v$ are real differentiable functions _and_ they satisfy the CRE.

## Application to Gravitational Potential
Let $V_y(y,z) := \partial_y V(y,z)$, and $V_{yy} := \partial^2_{yy}V(y,z)$, etc., denote the partial derivatives of the gravitational potential in the respective coordinate directions.


Due to the properties
$$\nabla \times \mathbf{g} = \mathbf{0},$$
and
$$\Delta V = 0,$$
the *Cauchy-Riemann* differential equations
$$
V_{yz} - V_{zy} = 0 \qquad \text{and} \qquad V_{yy} + V_{zz} = 0
$$
hold.

::: {.callout-note title="Correspondence between CR and gravity"}

| CR equations | Gravity components |
|--------|---------|
|  $x+iy$  | $z+iy$ |
| $u+iv$ | $V_y + i V_z$ |
| $u_x$ | $V_{yz}$ |
| $u_y$ | $V_{yy}$ |
| $v_x$ | $V_{zz}$ |
| $v_y$ | $V_{zy}$ |
| $u_x = v_y$ | $V_{yz} = V_{zy}$ |
| $u_y = -v_x$ | $V_{yy} = -V_{zz}$ |

:::


We may therefore assume that $V_y$ and $V_z$ are the real and imaginary parts of a complex function $G(s)$.

We say that $G(s)$ is _regular_ or _holomorphic_.

The functions $V_y$ and $V_z$ depend on $y$ and $z$, i.e., $V_y = V_y(y, z)$ and $V_z = V_z(y, z)$.


In the complex plane, the real coordinates $y$ and $z$ are combined into a complex coordinate $s = z + iy$.

Thus, we obtain the regular function $G : \mathbb{C} \to \mathbb{C}$
$$
G(s) = V_y(s) + i V_z(s).
$$


### Gravitational Acceleration in $\mathbb{R}$

With $r^2 = (y - y')^2 + (z - z')^2$, the components of the gravitational acceleration are given by
$$
V_y(y, z) = - 2 f \rho \iint_A \frac{y - y'}{r^2} \, dy' \, dz'
$$
and
$$
V_z(y, z) = - 2 f \rho \iint_A \frac{z - z'}{r^2} \, dy' \, dz'.
$$


### Gravitational Acceleration in $\mathbb{C}$

The gravitational acceleration in the complex plane can be expressed as
$$
G(s) = -2 f \rho i \iint_A \frac{1}{s - s'} \, dy' \, dz'.
$$

:::{.callout-note}

Note that with $s = z + iy$, $s' = z' + iy'$ follows

$$
s - s' = (z - z') + i(y - y').
$$
With complex conjugation we get
$$
\overline{s - s'} = (z - z') - i(y - y'),
$$
such that
$$
|s|^2 = s \cdot \overline{s}.
$$

:::

### Computation of $G$ in a Source-Free Region

Using the *Cauchy Integral Formula*, we find:
Let $G : \Omega \to \mathbb{C}$ be regular in a domain $\Omega$, and let $C : [a, b] \to \Omega \setminus \{z_0\}$ be a closed, positively oriented, piecewise $C^1$-continuous curve enclosing $z_0 \in \Omega$. Then,
$$
G(z_0) = \frac{1}{2 \pi i} \oint_C \frac{G(z)}{z - z_0} \, \mathrm{d}z.
$$
The values on the boundary completely determine those inside $C$.

If $z_0$ is located on $C$, then the CIF reduces to
$$
G(z_0) = \frac{1}{ \pi i} \oint_C \frac{G(z)}{z - z_0} \, \mathrm{d}z.
$$

### How to Choose the Integration Path?

By the *Cauchy Integral Theorem*, the integration path can be chosen arbitrarily. Since $G(s) \to 0$ as $y^2 + z^2 \to \infty$, $z < 0$, the integration path is chosen to fully encompass the $y$-axis, returning along an arc in the upper half-plane, extending to infinity.

![Choice of the integration path](images/contour_integral.excalidraw.svg){#fig-contour}

### Derivation of the Hilbert Transform

We separate real and imaginary parts of $G$ and obtain the *Hilbert Transform Pair*
$$
V_y(y) = +\frac{1}{\pi} \int\limits_{-\infty}^\infty \frac{V_z(y')}{y' - y} \, dy'
$$
and
$$
V_z(y) = -\frac{1}{\pi} \int\limits_{-\infty}^\infty \frac{V_y(y')}{y' - y} \, dy'.
$$


Recognizing these as convolution integrals:
$$
V_y(y) = -\frac{1}{\pi y} \ast V_z(y) = +\mathcal{H}\{V_z(y)\},
$$
and
$$
V_z(y) = +\frac{1}{\pi y} \ast V_y(y) = -\mathcal{H}\{V_y(y)\}.
$$

In the frequency domain, convolution becomes multiplication.

:::{.callout-note}
Note that
$$
\mathcal{H}(\mathcal{H}(u))(t) = -u(t),
$$
which follows from the effect of the Hilbert transform on the Fourier transform of $u(t)$ (see next section).
:::


### What is the Fourier Spectrum of $-\frac{1}{\pi y}$?


$$
-\frac{1}{\pi} \int\limits_{-\infty}^\infty \frac{e^{-i k y}}{y} \, dy = i \, \mathrm{sign}(k).
$$

Derivation using the *Residue Theorem in Complex Analysis*: Replace $\frac{1}{y}$ with $\lim_{a \to 0} \frac{y}{y^2 + a^2}$, $y = u + iv$, apply the Residue Theorem, and integrate around poles $+ia$ and $-ia$.

:::{.callout-note title="Fourier spectrum of the Hilbert transform operator"}
The goal is to find 
$$
\mathcal F\{ -\frac{1}{\pi y}, k\} = -\frac{1}{\pi} \int_{-\infty}^\infty \frac{e^{-i k y}}{y}\, \dd y.
$$
We replace $\frac{1}{y}$ with $\frac{y}{y^2 + a^2}$ and evaluate the integral in the limit
$$
\lim_{a \to 0} \int_{-\infty}^\infty \frac{y}{y^2 + a^2} e^{-i k y}\, \dd y.
$$
The integrand is a complex function of $y = u + iv$, hence
$$
e^{-iky}=e^{-iku}e^{+kv}
$$
The roots of the polynomial in the denominator are at $y=\pm ia$.

We use the residual theorem for a simple pole
$$
\text{Res} f(y) = \lim_{y \to y_{\text{pole}}}(y - y_{\text{pole}}) f(y) = \frac{1}{2 \pi i} \oint f(y) \, \dd y.
$$
Since the path of integration is arbitrary, we choose a path such that
$$
f(y) \to 0 \begin{cases} 
k<0 \text{ and } v \to +\infty \\
k<0 \text{ and } v \to -\infty
\end{cases}
$$

This reduces the integration to the real $y$-axis from $-\infty$ to $+\infty$.

![Path of integration around the pole at $y=-ia$.](images/integraton-hilbert.excalidraw.svg){#fig-integration-hilbert}

For $k<0$ we enclose the pole at $y=-ia$ and integrate clock-wise (sign!)
$$
\int_{-\infty}^\infty \frac{y}{y^2 + a^2} e^{-i k y}\, \dd y =
-\oint \frac{y}{y^2 + a^2} e^{-i k y}\, \dd y =
-2 \pi i \text{Res} f(y).
$$

$$
\begin{align}
-2 \pi i \text{Res}f(y) & = -2 \pi i \lim_{y \to -ia} (y+ia)f(y) \\
& = -2 \pi i \lim_{y \to -ia} (y+ia) \frac{y e^{-i k y}}{(y-ia)(y+ia)} \\
& = -2 \pi i \frac{-ia e^{+i^2 k a}}{-ia -ia} \\
& = -\pi i e^{-ka}
\end{align}
$$
Now
$$
\lim_{a\to 0} (- \pi i e^{-ka}) = -\pi i,
$$
which leads to the final result
$$
-\frac{1}{\pi} \int_{-\infty}^\infty \frac{e^{-i k y}}{y}\, \dd y = 
\begin{Bmatrix}
+i \qif k>0 \\
-i \qif k<0
\end{Bmatrix}
= i \, \text{sign}(k).
$$
:::

Thus, the spectrum of $-\frac{1}{\pi y}$ is $i \, \mathrm{sign}(k)$!

:::{.callout-important}

For negative and positive wave numbers $k$, the spectrum of $V_y$ (or $V_z$) is multiplied by $-i$ and $+i$, respectively.

:::

The Hilbert transform is a multiplier operator. The multiplier is $\Phi_H(k) = -i \, \mathrm{sign}(k)$, where $\mathrm{sign}$ is the signum function.

By Euler's formula,
$$
\Phi_H(k) =
\begin{cases}
+i = e^{+i\pi/2} & \qfor k < 0 \\
0 & \qfor k = 0 \\
-i = e^{-i\pi/2} & \qfor k > 0
\end{cases}
$$

The Hilbert transform has the effect of shifting the phase of the negative wavenumber components of the signal by +90$\textdegree$ and the phase of the positive wavenumber components by -90$\textdegree$.

When applied twice, the phase of the negative and positive wavenumber components are shifted by +180$\textdegree$ and -180$\textdegree$, resp., which are equivalent amounts. The signal is negated, because
$$
(\Phi_H(k))^2 = e^{\pm i \pi} = -1 \qfor k \ne 0.
$$

