---
title: "Solution of the Laplace equation in spherical coordinates"
---

Let $u: \mathbb R^3 \mapsto \mathbb R$ be a function defined in an open subset $\Omega \subset \mathbb R^3$.

Then $u$ is a solution to the Laplace equation, if 
$$
\Delta u = 0
$$
holds in $\Omega$.

We refer to $\Delta$ as the _Laplace operator_.

In different coordinate systems, $\Delta$ has different representations.

## Representations of the Laplace operator 

### Cartesian coordinates

$$
\frac{\partial^2 u}{\partial x^2}
+\frac{\partial^2 u}{\partial y^2}
+\frac{\partial^2 u}{\partial z^2}
= 0
$$ {#eq-laplace-cart}

### Spherical coordinates

![Spherical coordinate system](images/Kugelkoordinaten.excalidraw.svg){#fig-spherical}

We transform from a Cartesian to a spherical system with
$$
\begin{align}
x & = r \cos \phi \sin \theta \\
y & = r \sin \phi \sin \theta \\
z & = r \cos \theta \\
r^2 & = x^2 + y^2 + z^2
\end{align}
$$

$$
\frac{1}{r^2} \frac{\partial}{\partial r}
  \left( r^2 \frac{\partial u}{\partial r} \right) 
+ \frac{1}{r^2 \sin \theta} \frac{\partial}{\partial \theta}
  \left( \sin \theta {\partial u \over \partial \theta} \right) 
+ \frac{1}{r^2 \sin^2 \theta} \frac{\partial^2 u}{\partial \varphi^2} = 0
$$ {#eq-laplace-sph}

### Cylindrical coordinates

$$
\frac{1}{\rho} \frac{\partial}{\partial \rho}
  \left( \rho \frac{\partial u}{\partial \rho} \right) 
+ \frac{1}{\rho^2} \frac{\partial^2 u}{\partial \varphi^2}
+ \frac{\partial^2 u}{\partial z^2 } = 0
$$ {#eq-laplace-cyl}

$\rho^2 = x^2 + y^2$

### Polar coordinates

$$
\frac{1}{\rho} \frac{\partial}{\partial \rho}
  \left( \rho \frac{\partial u}{\partial \rho} \right) 
+ \frac{1}{\rho^2} \frac{\partial^2 u}{\partial \varphi^2} =0
$$ {#eq-laplace-polar}

$\rho^2 = x^2 + y^2$


## The radial part of the Laplace equation

We consider the Laplace equation in spherical coordinates as defined in @eq-laplace-sph.

For now, we assume that $u = u(r)$ is a function of the radial distance.

Thus, the Laplace equation reduces to an ordinary differential equation

$$
\frac{\mathrm d}{\mathrm d r}
  \left( r^2 \frac{\mathrm d u}{\mathrm d r} \right) =
  2r \frac{\mathrm d u}{\mathrm d r} + r^2 
  \frac{\mathrm d^2 u}{\mathrm d r^2} = 0.
$$

This equation is referred to as _Euler's differential equation_.

We solve this ODE with the _ansatz_
$$
u(r) = r^\alpha, \quad u'(r) = \alpha r ^{\alpha - 1}, \quad
 u''(r) = (\alpha-1)\alpha r^{\alpha - 2}.
$$

It follows
$$
\begin{align}
2r \alpha r^{\alpha-1} + r^2 (\alpha-1)\alpha r^{\alpha - 2} &= 0 \\
2 \alpha u + (\alpha-1)\alpha u &= 0 \\
\alpha(\alpha+1)u &= 0 \quad\text{(characteristic equation)}
\end{align}
$$

The characteristic equation has the solution
$$
u(r) = C_0 r^{-1} + C_1 r^0.
$$

At this point, we introduce the 

:::{.callout-note title="Homogeneous function"}

We call a function _homogeneous of degree $\lambda$_, if under a proportional scaling of the variables $x$ by a factor $t$ the function scales with a factor $t^\lambda$:

$$
f(t \mathbf x ) = t^\lambda f(\mathbf x)
$$

Example:

$f(x,y) = x^2 + y^2$ is a homogeneous function.

We replace $x$ and $y$ by $tx$ and $ty$, factor out powers of $t$, i.e.,
$$
f(tx, ty) = (tx)^2 + (ty)^2 = t^2(x^2 + y^2)
$$
and recognize that $f(x,y)$ is a homogeneous function of degree $2$.

:::

Now we make the following ansatz:

We assume that $u$ can be defined as a homogeneous function $u_n$ of dgree $n$. This is a valid choice, since homogeneous functions are solutions to Laplace's equation.

We set 
$$
\begin{align}
u_n(x,y,z) & = u_n(r \cos\phi \sin\theta, r \sin\phi \sin\theta, r \cos\theta) \\
& = r^n u_n(\cos\phi \sin\theta, \sin\phi \sin\theta,  \cos\theta) \\
& = r^n S_n(\phi, \theta)
\end{align}
$$

$u_n = r^n S_n(\phi, \theta)$ is a _spherical harmonic_.

Further,
$$
\begin{align}
2r  \frac{ \partial u_{n} }{ \partial r } 
 + r^2 \frac{ \partial^{2} u_{n} }{ \partial r^{2} } 
   & = 2 r n r^{n-1} S_n
  + r^2 n(n-1)r^{n-2} S_n \\
  & = 2 n u_n + n(n-1) u_n \\
  & = n(n+1) u_n
\end{align}
$$

We recognize that $f(r) = u_n(r)$ and $\lambda = n(n+1)$ are _eigenfunctions_ and _eigenvalues_ of the eigenvalue problem

$$
\Delta f(r) = \lambda f(r).
$$

We see that the radial part of the Laplace equation for $u_n$ can be equivalently replaced by
$$
n (n+1) u_n,
$$
which we insert back into the full Laplace equation @eq-laplace-sph to obtain

$$
n(n+1) S_n + \frac{1}{\sin \theta} \frac{\partial}{\partial \theta}
  \left( \sin \theta {\partial S_n \over \partial \theta} \right) 
+ \frac{1}{\sin^2 \theta} \frac{\partial^2 S_n}{\partial \varphi^2} = 0.
$$

## Zonal spherical harmonics

Now we seek solutions $S_n(\theta)$. These functions are referred to as _zonal spherical harmonics_. On a surface of a sphere they only vary with the polar angle $\theta$. Their zeros are parallel to the equator of the sphere.

The Laplace equation @eq-laplace-sph reduces to
$$
\frac{1}{\sin \theta} \frac{\mathrm d}{\mathrm d \theta}
  \left( \sin \theta {\mathrm d S_n \over \mathrm d \theta} \right) 
+ n(n+1) S_n = 0
$$

We substitute $\cos\theta$ and set $S_n(\theta)=P_n(t)$:

$$
\begin{align}
t & = \cos\theta \\
\mathrm{d}t & = -\sin \theta \,\mathrm{d}\theta \\
S_n(\theta) & = P_n(\cos\theta) = P_n(t)
\end{align} 
$$
With the chain rule we obtain
$$
\begin{align}
\frac{\mathrm d P_n(t)}{\mathrm d \theta} & = \frac{\mathrm d P_n(t)}{\mathrm d t} \frac{\mathrm d t}{\mathrm d \theta} \\
& = -\frac{\mathrm d P_n(t)}{\mathrm d t} \sin\theta \\
\sin^2\theta & = 1 - t^2
\end{align}
$$

Useful steps:
$$
\frac{1}{\sin \theta} \frac{\mathrm{d}}{\mathrm{d}\theta} =  
\frac{1}{\sin \theta} \left( -\frac{\sin \theta}{\mathrm{d}t} \right) = -\frac{\mathrm{d}}{\mathrm{d}t} 
$$

$$
\sin \theta \frac{\mathrm{d}}{\mathrm{d}\theta} =
\sin \theta \left( -\sin \theta \frac{\mathrm{d}}{\mathrm{d}t}  \right) = -\sin ^{2}\theta \frac{\mathrm{d}}{\mathrm{d}t} 
$$

Finally, we end at the _Legendre differential equation_

$$
\frac{\mathrm d}{\mathrm d t}
\left[
(1-t^2) \frac{\mathrm d P_n(t)}{\mathrm d t}
\right] + n(n+1) P_n(t) = 0
$$

The functions $P_n(t) = P_n(\cos\theta)$ are the _Legendre polynomials_.

When a pure dependency of $\theta$ is assumed, then
$$
r^{n} S_{n}(\theta) = r^{n} P_{n}(\cos \theta)
$$
and
$$
r^{-(n+1)}S_n = r^{-(n+1)}P_{n}(\cos \theta)
$$
are spherical harmonics.

## The angular component of the Laplace equation

Previously, we have encountered zonal spherical harmonics or Legendre polynomials as solutions to the Laplace equation.

Formally, the zonal spherical harmonics $S_n(\theta) = P_n(\cos\theta)$ correspond to the Legendre polynomials.

To arrive at $S_n(\theta, \phi)$, we use a *separation of variables* approach of the form:

$$S_n(\theta, \phi) = \Theta(\theta)\Phi(\phi)$$

and write:

$$
\underbrace{ n(n+1)\Theta\Phi + \frac{\Phi}{\sin\theta}\frac{\mathrm d}{\mathrm d \theta}\left(\sin\theta \frac{\mathrm d \Theta}{\mathrm d \theta}\right) }_{ =m^{2} } +
\underbrace{ \frac{\Theta}{\sin^2\theta}\frac{\mathrm d^2 \Phi}{\mathrm d \phi^2} }_{ =-m^{2} }
=0
$$

or, after multiplying by $\dfrac{\sin^{2}\theta}{\Theta \Phi}$:

$$
n(n+1) \sin^2\theta + \frac{\sin\theta}{\Theta} \frac{\mathrm d}{\mathrm d \theta}
\left(\sin\theta \frac{\mathrm d \Theta}{\mathrm d \theta}\right) = m^2
$$

$$\frac{1}{\Phi} \frac{\mathrm d^2 \Phi}{\mathrm d \phi^2} = -m^2$$

Solutions can be provided for both equations.

First, we consider:

$$\Phi''+m^2 \Phi = 0$$

This is a harmonic differential equation with the solution:

$$
\Phi(\phi) = A_m \cos m \phi + B_m \sin m \phi
$$

The other equation is:

$$\dfrac{1}{\sin\theta}\frac{\mathrm d}{\mathrm d \theta}
\left(\sin\theta \frac{\mathrm d \Theta}{\mathrm d \theta}\right) + 
\left[
n(n+1) - \frac{m^2}{\sin^2\theta}
\right]\Theta = 0$$

We seek the solution $\Theta(\theta)$, substitute $t = \cos\theta$, $\mathrm d t = -\sin\theta \mathrm d\theta$, and assume $\Theta(\theta) = P_n^m(\cos\theta) = P_n^m(t)$. Thus:

$$\frac{\mathrm d}{\mathrm d t}
\left[
(1-t^2) \frac{\mathrm d P_n^m(t)}{\mathrm d t}
\right] +
\left[
n(n+1) - \frac{m^2}{1-t^2}
\right] P_n^m(t) = 0$$

The desired $P_n^m(t)$ are *associated Legendre functions* of order $m$ and degree $n$.

The associated Legendre functions can be most easily defined through the derivatives of the Legendre polynomials with $0 \le m \le n$:

$$
\begin{align}
P_n^m(t) & = (1 - t^2)^{\frac{m}{2}} \frac{\mathrm d^m}{\mathrm dt^m}P_n(t)  \\
P_n^m(\cos \theta)  & = \sin ^{m}\theta P_n^{(m)}(\cos \theta)
\end{align}
$$

where $P_{n}^{(m)}$ is the $m$-th derivative of $P_{n}$ with respect to $\cos \theta$.
